theories/rules/rules_Jmp.v
@@ -2,24 +2,183 @@ From iris.base_logic Require Export invariants gen_heap.
 From iris.program_logic Require Export weakestpre ectx_lifting.
 From iris.proofmode Require Import proofmode.
 From iris.algebra Require Import frac.
-From cap_machine Require Export rules_base.
+From cap_machine Require Export rules_base register_tactics.
 
 Section cap_lang_rules.
   Context `{memG Σ, regG Σ}.
   Context `{MachineParameters}.
   Implicit Types P Q : iProp Σ.
   Implicit Types σ : ExecConf.
-  Implicit Types c : cap_lang.expr. 
+  Implicit Types c : cap_lang.expr.
   Implicit Types a b : Addr.
   Implicit Types r : RegName.
-  Implicit Types v : cap_lang.val. 
+  Implicit Types v : cap_lang.val.
   Implicit Types w : Word.
   Implicit Types reg : gmap RegName Word.
   Implicit Types ms : gmap Addr Word.
 
+  Inductive Jmp_failure (regs: Reg) (r: RegName) (mem : gmap Addr Word) :=
+  | Jmp_fail_bounds b e a:
+      regs !! r = Some (WCap IE b e a) ->
+      (withinBounds b e a = false \/ withinBounds b e (a^+1)%a = false) →
+      Jmp_failure regs r mem
+  .
+
+  Inductive Jmp_spec
+    (regs: Reg) (r: RegName)
+    (regs': Reg) (mem : gmap Addr Word) : cap_lang.val → Prop
+  :=
+  | Jmp_spec_success_IE b e a wpc wddc :
+    regs !! r = Some (WCap IE b e a) ->
+    withinBounds b e a = true ->
+    withinBounds b e (a^+1)%a = true ->
+    mem !! a = Some wpc ->
+    mem !! (a^+1)%a = Some wddc ->
+    regs' = ( <[ ddc := wddc ]> (<[ PC := wpc ]> regs)) ->
+    Jmp_spec regs r regs' mem NextIV
+
+  | Jmp_spec_success w :
+    regs !! r = Some w ->
+    (forall p b e a, w = WCap p b e a -> p <> IE) ->
+    regs' = <[ PC := updatePcPerm w]> regs ->
+    Jmp_spec regs r regs' mem NextIV
+
+  | Jmp_spec_failure :
+    Jmp_failure regs r mem ->
+    Jmp_spec regs r regs' mem FailedV.
+
+  Definition allow_load_map_or_true r (regs : Reg) (mem : gmap Addr Word):=
+    ∃ p b e a,
+      read_reg_inr regs r p b e a ∧
+        if decide
+             (regs !! r = Some (WCap p b e a)
+              /\ withinBounds b e a = true
+              /\ withinBounds b e (a^+1)%a = true)
+        then
+          (∃ w, mem !! a = Some w) /\ (∃ w, mem !! (a^+1)%a = Some w)
+        else True.
+
+  Lemma wp_jmp
+    Ep pc_p pc_b pc_e pc_a
+    r w mem regs  :
+    decodeInstrW w = Jmp r →
+    isCorrectPC (WCap pc_p pc_b pc_e pc_a) →
+
+    regs !! PC = Some (WCap pc_p pc_b pc_e pc_a) →
+    ( forall b' e' a', regs !! r = Some (WCap IE b' e' a') ->
+                  is_Some (regs !! ddc) /\ allow_load_map_or_true r regs mem)->
+    regs_of (Jmp r) ⊆ dom regs →
+    mem !! pc_a = Some w →
+
+
+    {{{ (▷ [∗ map] a↦w ∈ mem, a ↦ₐ w) ∗
+          ▷ [∗ map] k↦y ∈ regs, k ↦ᵣ y }}}
+      Instr Executable @ Ep
+      {{{ regs' retv, RET retv;
+          ⌜ Jmp_spec regs r regs' mem retv⌝ ∗
+            ([∗ map] a↦w ∈ mem, a ↦ₐ w) ∗
+            [∗ map] k↦y ∈ regs', k ↦ᵣ y }}}.
+  Proof.
+    iIntros (Hinstr Hvpc HPC HDDC Dregs Hmem_pc φ) "(>Hmem & >Hmap) Hφ".
+    iApply wp_lift_atomic_head_step_no_fork; auto.
+    iIntros (σ1 ns l1 l2 nt) "[Hr Hm] /=". destruct σ1; simpl.
+    iDestruct (gen_heap_valid_inclSepM with "Hr Hmap") as %Hregs.
+
+    (* Derive necessary register values in r *)
+    pose proof (lookup_weaken _ _ _ _ HPC Hregs).
+    specialize (indom_regs_incl _ _ _ Dregs Hregs) as Hri. unfold regs_of in Hri.
+    feed destruct (Hri r) as [rv [Hr' _]]. by set_solver+. clear Hri.
+    (* Derive the PC in memory *)
+    iDestruct (gen_mem_valid_inSepM mem m with "Hm Hmem") as %Hma; eauto.
+
+    iModIntro.
+    iSplitR. by iPureIntro; apply normal_always_head_reducible.
+    iNext. iIntros (e2 σ2 efs Hpstep).
+    apply prim_step_exec_inv in Hpstep as (-> & -> & (c & -> & Hstep)).
+    iIntros "_".
+    iSplitR; auto. eapply step_exec_inv in Hstep; eauto.
+
+    rewrite /exec /= in Hstep.
+
+    (* Now we start splitting on the different cases in the Jmp spec, and prove them one at a time *)
+    assert (Hr0 : r0 !! r = Some rv).
+    { eapply (lookup_weaken regs r0) ;auto. }
+    destruct (is_cap rv) eqn:Hrv.
+    - (* rv is a capability, we need to destruct on permission *)
+      destruct rv; simpl in Hrv; try discriminate.
+      destruct sb as [ p b e a |]; simpl in Hrv; try discriminate ; clear Hrv.
+      destruct (decide (p = IE)) as [Hp | Hp].
+      + (* p = IE, we need to make sure that *)
+        destruct (decide (withinBounds b e a && withinBounds b e (a ^+ 1)%a)) as
+          [Hbounds%Is_true_true | Hbounds%Is_true_false]
+          ; (rewrite Hr0 /= Hbounds /= in Hstep).
+        * (* in bounds, success *)
+        destruct p; simpl; simplify_pair_eq.
+        pose proof Hr' as Hr.
+        apply HDDC in Hr; clear HDDC.
+        destruct Hr as [HDDC HaLoad].
+        unfold allow_load_map_or_true in HaLoad.
+        destruct HaLoad as (p' & b' & e' & a' & Hread_reg & HaLoad).
+        unfold read_reg_inr in Hread_reg.
+        rewrite Hr' in Hread_reg. injection Hread_reg ; intros ; subst
+        ; clear Hread_reg.
+
+        case_decide.
+        2: { (* contradiction *)
+          exfalso.
+          apply andb_true_iff in Hbounds.
+          apply H3; split ; auto.
+        }
+        destruct HaLoad as [[wpc Ha] [wddc Ha']].
+
+        iDestruct (gen_mem_valid_inSepM mem m a' wpc with "Hm Hmem" ) as %Hma'
+        ; eauto.
+
+        iDestruct (gen_mem_valid_inSepM mem m (a'^+1)%a wddc with "Hm Hmem" ) as %Hma''
+        ; eauto.
+        rewrite Hma' Hma'' /= in Hstep.
+
+        simpl; simplify_pair_eq.
+        iMod ((gen_heap_update_inSepM _ _ PC wpc) with "Hr Hmap") as "[Hr Hmap]"; eauto.
+        iMod ((gen_heap_update_inSepM _ _ ddc wddc) with "Hr Hmap") as
+          "[Hr Hmp]" ; eauto.
+        { apply lookup_insert_is_Some'; by right. }
+        iFrame; try iApply "Hφ"; iFrame.
+        apply andb_true_iff in Hbounds ; destruct Hbounds as [Hbounds_a Hbounds_a'].
+        iPureIntro; eapply Jmp_spec_success_IE; eauto.
+
+        * (* in bounds, failure *)
+          destruct p; simpl; simplify_pair_eq.
+          iFrame; try iApply "Hφ"; iFrame.
+          iPureIntro; eapply Jmp_spec_failure ; econstructor ; eauto.
+          by apply andb_false_iff.
+
+
+      + (* p <> IE, so it doesn't fail *)
+        (* Success *)
+        rewrite Hr0 /= in Hstep.
+        destruct p; simpl; simplify_pair_eq
+        ; iMod ((gen_heap_update_inSepM _ _ PC) with "Hr Hmap") as "[Hr Hmap]"
+        ; eauto
+        ; iFrame; try iApply "Hφ"; iFrame
+        ; iPureIntro; eapply Jmp_spec_success; eauto
+        ; intros * Hcontra ; injection Hcontra
+        ; intros _ _ _ Hcontra' ; clear -Hcontra'; subst ; congruence.
+    - (* rv is not capability, always success *)
+      (* Success *)
+      destruct rv; simpl in Hrv
+      ; try (destruct sb; simpl in Hrv; try discriminate ; clear Hrv)
+      ; rewrite Hr0 /= in Hstep; simplify_pair_eq
+      ; try (iMod ((gen_heap_update_inSepM _ _ PC) with "Hr Hmap") as "[Hr Hmap]"
+      ; eauto
+      ; iFrame; try iApply "Hφ"; iFrame
+      ; iPureIntro; eapply Jmp_spec_success; eauto).
+  Qed.
+
   Lemma wp_jmp_success E pc_p pc_b pc_e pc_a w r w' :
     decodeInstrW w = Jmp r →
      isCorrectPC (WCap pc_p pc_b pc_e pc_a) →
+     (forall b e a, w' <> WCap IE b e a) ->
 
      {{{ ▷ PC ↦ᵣ WCap pc_p pc_b pc_e pc_a
          ∗ ▷ pc_a ↦ₐ w
@@ -30,22 +189,31 @@ Section cap_lang_rules.
            ∗ pc_a ↦ₐ w
            ∗ r ↦ᵣ w' }}}.
   Proof.
-    iIntros (Hinstr Hvpc ϕ) "(>HPC & >Hpc_a & >Hr) Hφ".
-    iApply wp_lift_atomic_head_step_no_fork; auto.
-    iIntros (σ1 ns l1 l2 nt) "Hσ1 /=". destruct σ1; simpl.
-    iDestruct "Hσ1" as "[Hr0 Hm]".
-    iDestruct (@gen_heap_valid with "Hm Hpc_a") as %?; auto.
-    iDestruct (@gen_heap_valid with "Hr0 HPC") as %?.
-    iDestruct (@gen_heap_valid with "Hr0 Hr") as %Hr_r0.
-    iModIntro. iSplitR. by iPureIntro; apply normal_always_head_reducible.
-    iNext. iIntros (e2 σ2 efs Hpstep).
-    apply prim_step_exec_inv in Hpstep as (-> & -> & (c & -> & Hstep)).
-    iIntros "_".
-    iSplitR; auto. eapply step_exec_inv in Hstep; eauto.
-    unfold exec, exec_opt in Hstep. rewrite Hr_r0 /= in Hstep. simplify_pair_eq.
+    iIntros (Hinstr Hvpc Hw' ϕ) "(>HPC & >Hpc_a & >Hr) Hφ".
 
-    iMod (@gen_heap_update with "Hr0 HPC") as "[Hr0 HPC]". iFrame.
-    iApply "Hφ". by iFrame.
+    iDestruct (memMap_resource_1 with "Hpc_a") as "Hmem".
+    iDestruct (map_of_regs_2 with "HPC Hr") as "[Hreg %Hr]".
+    iApply (wp_jmp with "[$Hmem $Hreg]"); eauto ; simplify_map_eq; eauto.
+    { intros * Hcontra; injection Hcontra ; intros ; subst.
+      specialize (Hw' b' e' a') ; congruence. }
+    { by rewrite !dom_insert; set_solver+. }
+
+    iNext.
+    iIntros (regs retv) "(%& Hmem & Hreg)".
+    inversion H2; simplify_map_eq.
+    - (* Success IE - contradiction *)
+      specialize (Hw' b e a) ; congruence.
+    - (* Success not IE *)
+      iExtractList "Hreg" [PC;r] as ["HPC"; "Hr"].
+      iDestruct (big_sepM_insert with "Hmem") as "[Hpc_a _]"; auto.
+      iApply "Hφ" ; iFrame.
+    - (* Failure - contradiction *)
+      exfalso.
+      inversion H3.
+      rewrite (_: <[PC:=WCap pc_p pc_b pc_e pc_a]> (<[r:=w']> ∅) !! r = Some w')
+        in H4 ; [| by simplify_map_eq].
+      injection H4 ; intros ->.
+      specialize (Hw' b e a) ; congruence.
   Qed.
 
   Lemma wp_jmp_successPC E pc_p pc_b pc_e pc_a w :
@@ -60,20 +228,95 @@ Section cap_lang_rules.
            ∗ pc_a ↦ₐ w }}}.
   Proof.
     iIntros (Hinstr Hvpc ϕ) "(>HPC & >Hpc_a) Hφ".
-    iApply wp_lift_atomic_head_step_no_fork; auto.
-    iIntros (σ1 ns l1 l2 nt) "Hσ1 /=". destruct σ1; cbn.
-    iDestruct "Hσ1" as "[Hr0 Hm]".
-    iDestruct (@gen_heap_valid with "Hm Hpc_a") as %?; auto.
-    iDestruct (@gen_heap_valid with "Hr0 HPC") as %Hr_PC.
-    iModIntro. iSplitR. by iPureIntro; apply normal_always_head_reducible.
-    iNext. iIntros (e2 σ2 efs Hpstep).
-    apply prim_step_exec_inv in Hpstep as (-> & -> & (c & -> & Hstep)).
-    iIntros "_".
-    iSplitR; auto. eapply step_exec_inv in Hstep; eauto.
-    unfold exec, exec_opt in Hstep. rewrite Hr_PC /= in Hstep. simplify_pair_eq.
 
-    iMod (@gen_heap_update with "Hr0 HPC") as "[Hr0 HPC]". iFrame.
-    iApply "Hφ". by iFrame.
+    iDestruct (memMap_resource_1 with "Hpc_a") as "Hmem".
+    iDestruct (map_of_regs_1 with "HPC") as "Hreg".
+    iApply (wp_jmp with "[$Hmem $Hreg]"); eauto ; simplify_map_eq; eauto.
+    { intros * Hcontra; injection Hcontra ; intros ; subst.
+      inversion Hvpc ; destruct H7 ; congruence. }
+    { by rewrite !dom_insert; set_solver+. }
+
+    iNext.
+    iIntros (regs retv) "(%& Hmem & Hreg)".
+    inversion H2; simplify_map_eq.
+    - (* Success IE - contradiction *)
+      inversion Hvpc ; destruct H11 ; congruence.
+    - (* Success not IE *)
+      iExtractList "Hreg" [PC] as ["HPC"].
+      iDestruct (big_sepM_insert with "Hmem") as "[Hpc_a _]"; auto.
+      iApply "Hφ" ; iFrame.
+    - (* Failure - contradiction *)
+      exfalso.
+      inversion H3.
+      simplify_map_eq.
+      inversion Hvpc ; destruct H10 ; congruence.
+  Qed.
+
+
+  (* TODO we need to do cases where:
+       - r = ddc
+       - pc_a = a
+       - pc_a = a+1
+   *)
+  Lemma wp_jmp_success_IE E pc_p pc_b pc_e pc_a w r b e a w' wpc wddc :
+    decodeInstrW w = Jmp r →
+     isCorrectPC (WCap pc_p pc_b pc_e pc_a) →
+     withinBounds b e a = true ->
+     withinBounds b e (a^+1)%a = true ->
+     r <> ddc ->
+
+     {{{ ▷ PC ↦ᵣ WCap pc_p pc_b pc_e pc_a
+         ∗ ▷ r ↦ᵣ WCap IE b e a
+         ∗ ▷ ddc ↦ᵣ w'
+         ∗ ▷ pc_a ↦ₐ w
+         ∗ ▷ a ↦ₐ wpc
+         ∗ ▷ (a^+1)%a ↦ₐ wddc
+     }}}
+       Instr Executable @ E
+       {{{ RET NextIV;
+           PC ↦ᵣ wpc
+         ∗ r ↦ᵣ WCap IE b e a
+         ∗ ddc ↦ᵣ wddc
+         ∗ pc_a ↦ₐ w
+         ∗ a ↦ₐ wpc
+         ∗ (a^+1)%a ↦ₐ wddc }}}.
+    Proof.
+    iIntros (Hinstr Hvpc Hbound_a Hbound_a' Hr ϕ)
+      "(>HPC  & >Hr & >Hddc & >Hpc_a & >Ha & >Ha') Hφ".
+
+    iDestruct (address_neq with "Ha' Hpc_a") as "%Ha'".
+    iDestruct (address_neq with "Ha Ha'") as "%Hneqa".
+    iDestruct (memMap_resource_2ne_apply with "Hpc_a Ha") as "[Hmem %Ha]".
+    iDestruct (big_sepM_insert with "[Ha' Hmem]") as "Hmem" ; [| iFrame |].
+    by simplify_map_eq.
+    iDestruct (map_of_regs_3 with "HPC Hr Hddc") as "[Hreg %Hr']".
+    destruct Hr' as (?&?&?).
+    iApply (wp_jmp with "[$Hmem $Hreg]"); eauto ; simplify_map_eq; eauto.
+    { intros * Hreg_r; simplify_map_eq.
+      split ; auto.
+      unfold allow_load_map_or_true. exists IE, b', e', a'.
+      split.
+      unfold read_reg_inr; by simplify_map_eq.
+      case_decide as H' ; auto ; clear H'.
+      split ; eexists ; by simplify_map_eq. }
+    { by rewrite !dom_insert; set_solver+. }
+
+    iNext.
+    iIntros (regs retv) "(%Hspec& Hmem & Hreg)".
+    inversion Hspec; simplify_map_eq.
+    - (* Success IE *)
+      iApply "Hφ".
+      iExtractList "Hreg" [PC;ddc;r] as ["HPC"; "Hddc" ; "Hr"].
+      iDestruct (big_sepM_insert with "Hmem") as "[Ha' Hmem]"; auto ; [ by simplify_map_eq|].
+      iDestruct (big_sepM_insert with "Hmem") as "[Hpc_a Hmem]"; auto ; [ by simplify_map_eq|].
+      iDestruct (big_sepM_insert with "Hmem") as "[Ha _]"; auto.
+      iFrame.
+    - (* Success not IE - contradiction *)
+      exfalso ; by eapply H6.
+    - (* Failure - contradiction *)
+      exfalso.
+      inversion H5; simplify_map_eq.
+      destruct H7; congruence.
   Qed.
 
 End cap_lang_rules.
